Change to use immutables objects.

simple_tm.dfy
@@ -16,19 +16,19 @@ module ModelingTM {
     // Process state : transaction progress and process memory.
     class ProcessState {
         // currentTx : id of tx being processed. txs.size() means done.
-        var currentTx: nat
+        const currentTx: nat
         // currentOp :
         //      - tx.ops.size() represents tryCommit operation.
         //      - -1 represents abort operation
         //      - values in between represent read and write operations
-        var currentOp: int
+        const currentOp: int
         // sub-operations of the operation, see the step function
-        var currentSubOp: nat
+        const currentSubOp: nat
 
         // Set of read objects with original observed timestamp.
-        var readSet: map<MemoryObject, TimeStamp>
+        const readSet: map<MemoryObject, TimeStamp>
         // Set of read objects with original observed value.
-        var writeSet: map<MemoryObject, MemoryObjectValue>
+        const writeSet: map<MemoryObject, MemoryObjectValue>
 
         constructor () {
             currentTx := 0;
@@ -37,168 +37,426 @@ module ModelingTM {
             readSet := map[];
             writeSet := map[];
         }
+
+        constructor nextSubOp(that: ProcessState)
+            ensures this.currentTx == that.currentTx
+            ensures this.currentOp == that.currentOp
+            ensures this.currentSubOp == that.currentSubOp + 1
+            ensures this.readSet == that.readSet
+            ensures this.writeSet == that.writeSet
+        {
+            currentTx := that.currentTx;
+            currentOp := that.currentOp;
+            currentSubOp := that.currentSubOp + 1;
+            readSet := that.readSet;
+            writeSet := that.writeSet;
+        }
+
+        constructor nextOp(that: ProcessState)
+            ensures this.currentTx == that.currentTx
+            ensures this.currentOp == that.currentOp + 1
+            ensures this.currentSubOp == 0
+            ensures this.readSet == that.readSet
+            ensures this.writeSet == that.writeSet
+        {
+            currentTx := that.currentTx;
+            currentOp := that.currentOp + 1;
+            currentSubOp := 0;
+            readSet := that.readSet;
+            writeSet := that.writeSet;
+        }
+
+        constructor abortTx(that: ProcessState)
+            ensures this.currentTx == that.currentTx
+            ensures this.currentOp == -1
+            ensures this.currentSubOp == 0
+            ensures this.readSet == that.readSet
+            ensures this.writeSet == that.writeSet
+        {
+            currentTx := that.currentTx;
+            currentOp := -1;
+            currentSubOp := 0;
+            readSet := that.readSet;
+            writeSet := that.writeSet;
+        }
+
+        constructor restartTx(that: ProcessState)
+            ensures this.currentTx == that.currentTx
+            ensures this.currentOp == 0
+            ensures this.currentSubOp == 0
+            ensures this.readSet == map[]
+            ensures this.writeSet == map[]
+        {
+            currentTx := that.currentTx;
+            currentOp := 0;
+            currentSubOp := 0;
+            readSet := map[];
+            writeSet := map[];
+        }
+
+        constructor nextTx(that: ProcessState)
+            ensures this.currentTx == that.currentTx + 1
+            ensures this.currentOp == 0
+            ensures this.currentSubOp == 0
+            ensures this.readSet == map[]
+            ensures this.writeSet == map[]
+        {
+            currentTx := that.currentTx + 1;
+            currentOp := 0;
+            currentSubOp := 0;
+            readSet := map[];
+            writeSet := map[];
+        }
+
+        constructor addToReadSet(that: ProcessState, obj: MemoryObject, ts: TimeStamp)
+            ensures currentTx == that.currentTx
+            ensures currentOp == that.currentOp
+            ensures currentSubOp == that.currentSubOp
+            ensures readSet.Keys == that.readSet.Keys + {obj}
+                && readSet[obj] == ts
+                && forall o :: o in readSet && o != obj ==> readSet[o] == that.readSet[o]
+            ensures writeSet == that.writeSet
+        {
+            currentTx := that.currentTx;
+            currentOp := that.currentOp;
+            currentSubOp := that.currentSubOp;
+            readSet := that.readSet[obj := ts];
+            writeSet := that.writeSet;
+        }
+
+        constructor addToWriteSet(that: ProcessState, obj: MemoryObject, v: MemoryObjectValue)
+            ensures this.currentTx == that.currentTx
+            ensures this.currentOp == that.currentOp
+            ensures this.currentSubOp == that.currentSubOp
+            ensures this.readSet == that.readSet
+            ensures this.writeSet.Keys == that.writeSet.Keys + {obj}
+                && this.writeSet[obj] == v
+                && forall o :: o in writeSet && o != obj ==> writeSet[o] == that.writeSet[o]
+        {
+            currentTx := that.currentTx;
+            currentOp := that.currentOp;
+            currentSubOp := that.currentSubOp;
+            readSet := that.readSet;
+            writeSet := that.writeSet[obj := v];
+        }
     }
 
     class TMSystem {
-        const procs: set<ProcessId>
         // Ordered list of transaction that each process should process
         const txQueues : map<ProcessId, seq<Transaction>>
         // State and memory of processes
-        var procStates : map<ProcessId, ProcessState>
+        const procStates : map<ProcessId, ProcessState>
         // Value of object (not actually necessary for the proofs)
-        var objValues: map<MemoryObject, MemoryObjectValue>
+        const objValues: map<MemoryObject, MemoryObjectValue>
         // Object lock.
-        var lockedObjs: set<MemoryObject>
+        const lockedObjs: set<MemoryObject>
         // Object timestamp. (Incremented at the end of any write transaction)
-        var objTimeStamps: map<MemoryObject, nat>
+        const objTimeStamps: map<MemoryObject, nat>
 
         constructor (q: map<ProcessId, seq<Transaction>>) {
             txQueues := q;
-            var temp : map<ProcessId, ProcessState>  := map[];
             procStates := map[];
             objValues := map[];
             lockedObjs := {};
             objTimeStamps := map[];
         }
 
-        method Step(p: ProcessId, state: ProcessState)
-            requires p in txQueues
-            requires p in procStates && procStates[p] == state
-            modifies this
-            modifies state
+        constructor initValue(that: TMSystem, obj: MemoryObject)
+            ensures txQueues == that.txQueues
+            ensures procStates == that.procStates
+            ensures objValues.Keys == that.objValues.Keys + {obj}
+                && objValues[obj] == 0
+                && forall o :: o in objValues && o != obj ==> objValues[o] == that.objValues[o]
+            ensures lockedObjs == that.lockedObjs
+            ensures objTimeStamps.Keys ==  that.objTimeStamps.Keys + {obj}
+                && objTimeStamps[obj] == 0
+                && forall o :: o in objTimeStamps && o != obj ==> objTimeStamps[o] == that.objTimeStamps[o]
         {
-            var txs := txQueues[p];
-            if(!(p in procStates)) {
-                var newState :=  new ProcessState();
-                procStates := procStates[p := newState];
-            }
-            if (state.currentTx >= |txs|) {
-                // Nothing left to do.
-                return;
-            }
-            var tx := txs[state.currentTx];
-            if (state.currentOp == |tx.ops|) {
-                // tryCommit
-                if(state.currentSubOp == 0) {
-                    // Validate timestamps
-                    if !(forall o :: o in state.readSet ==> state.readSet[o] == objTimeStamps[o]) {
-                        // Write detected (timestamp changed), aborting.
-                        state.currentOp := -1;
-                        state.currentSubOp := 0;
-                        return;
-                    }
-                    // Continue to next sub-op.
-                    state.currentSubOp := state.currentSubOp + 1;
-                } else if (state.currentSubOp == 1) {
-                    // Check locks
-                    if !(forall o :: o in state.readSet ==> o in state.writeSet || o !in lockedObjs) {
-                        // Write detected (locked), aborting.
-                        state.currentOp := -1;
-                        state.currentSubOp := 0;
-                        return;
-                    }
-                    // Can commit ! Continue to next sub-op.
-                    state.currentSubOp := state.currentSubOp + 1;
-                } else if (state.currentSubOp == 2) {
-                    // Update timestamps
-                    objTimeStamps := map o | o in objTimeStamps ::
-                        if(o in state.writeSet) then (objTimeStamps[o] + 1) else objTimeStamps[o];
-                    // Continue to next sub-op.
-                    state.currentSubOp := state.currentSubOp + 1;
-                } else if (state.currentSubOp == 3) {
-                    // Release locks
-                    lockedObjs := lockedObjs - state.writeSet.Keys;
-                    state.writeSet := map[];
-                    state.readSet := map[];
-                    // Commited. Continue to next transaction.
-                    state.currentTx := state.currentTx + 1;
-                    state.currentOp := 0;
-                    state.currentSubOp := 0;
+            txQueues := that.txQueues;
+            procStates := that.procStates;
+            objValues := that.objValues[obj := 0];
+            lockedObjs := that.lockedObjs;
+            objTimeStamps := that.objTimeStamps[obj := 0];
+        }
+        
+        constructor updateState(that: TMSystem, pid: ProcessId, state: ProcessState)
+            ensures txQueues == that.txQueues
+            ensures procStates.Keys == that.procStates.Keys + {pid}
+                && procStates[pid] == state
+                && forall p :: p in procStates && p != pid ==> procStates[p] == that.procStates[p]
+            ensures objValues == that.objValues
+            ensures lockedObjs == that.lockedObjs
+            ensures objTimeStamps ==  that.objTimeStamps
+        {
+            txQueues := that.txQueues;
+            procStates := that.procStates[pid := state];
+            objValues := that.objValues;
+            lockedObjs := that.lockedObjs;
+            objTimeStamps := that.objTimeStamps;
+        }
+        
+        constructor updateValue(that: TMSystem, obj: MemoryObject, v: MemoryObjectValue)
+            ensures txQueues == that.txQueues
+            ensures procStates == that.procStates
+            ensures objValues.Keys == that.objValues.Keys + {obj}
+                && objValues[obj] == v
+                && forall o :: o in objValues && o != obj ==> objValues[o] == that.objValues[o]
+            ensures lockedObjs == that.lockedObjs
+            ensures objTimeStamps ==  that.objTimeStamps
+        {
+            txQueues := that.txQueues;
+            procStates := that.procStates;
+            objValues := that.objValues[obj := v];
+            lockedObjs := that.lockedObjs;
+            objTimeStamps := that.objTimeStamps;
+        }
+        
+        constructor restoreValues(that: TMSystem, original: map<MemoryObject, MemoryObjectValue>)
+            ensures txQueues == that.txQueues
+            ensures procStates == that.procStates
+            ensures objValues.Keys == that.objValues.Keys
+                && forall o :: o in objValues ==>
+                    if(o in original) then objValues[o] == original[o] else objValues[o] == that.objValues[o]
+            ensures lockedObjs == that.lockedObjs
+            ensures objTimeStamps ==  that.objTimeStamps
+        {
+            txQueues := that.txQueues;
+            procStates := that.procStates;
+            objValues := map o | o in that.objValues :: if (o in original) then original[o] else that.objValues[o];
+            lockedObjs := that.lockedObjs;
+            objTimeStamps := that.objTimeStamps;
+        }
+
+        constructor acquireLock(that: TMSystem, o: MemoryObject)
+            ensures txQueues == that.txQueues
+            ensures procStates == that.procStates
+            ensures objValues == that.objValues
+            ensures lockedObjs == that.lockedObjs + {o}
+            ensures objTimeStamps == that.objTimeStamps
+        {
+            txQueues := that.txQueues;
+            procStates := that.procStates;
+            objValues := that.objValues;
+            lockedObjs := that.lockedObjs + {o};
+            objTimeStamps := that.objTimeStamps;
+        }
+
+        constructor releaseLocks(that: TMSystem, objs: set<MemoryObject>)
+            ensures txQueues == that.txQueues
+            ensures procStates == that.procStates
+            ensures objValues == that.objValues
+            ensures lockedObjs == that.lockedObjs - objs
+            ensures objTimeStamps ==  that.objTimeStamps
+        {
+            txQueues := that.txQueues;
+            procStates := that.procStates;
+            objValues := that.objValues;
+            lockedObjs := that.lockedObjs - objs;
+            objTimeStamps := that.objTimeStamps;
+        }
+        
+        constructor updateTimestamps(that: TMSystem, objs: set<MemoryObject>)
+            ensures txQueues == that.txQueues
+            ensures procStates == that.procStates
+            ensures objValues == that.objValues
+            ensures lockedObjs == that.lockedObjs
+            ensures objTimeStamps.Keys == that.objTimeStamps.Keys
+                && forall o :: o in that.objTimeStamps ==>
+                if(o in objs) then objTimeStamps[o] != that.objTimeStamps[o] else objTimeStamps[o] == that.objTimeStamps[o]
+        {
+            txQueues := that.txQueues;
+            procStates := that.procStates;
+            objValues := that.objValues;
+            lockedObjs := that.lockedObjs;
+            objTimeStamps := map o | o in that.objTimeStamps ::
+                if(o in objs) then (that.objTimeStamps[o] + 1) else that.objTimeStamps[o];
+        }
+
+        predicate stateValid(pid: ProcessId, state: ProcessState)
+            requires pid in procStates && state == procStates[pid]
+        {
+            && pid in txQueues
+            && state.currentTx <= |txQueues[pid]|
+            && if state.currentTx == |txQueues[pid]| then (
+                // Queue finished
+                && state.currentOp == 0
+                && state.currentSubOp == 0
+                && |state.readSet| == 0
+                && |state.writeSet| == 0
+            ) else if state.currentTx < |txQueues[pid]| then (
+                // Queue unfinished
+                && exists tx :: (
+                    && tx == txQueues[pid][state.currentTx]
+                    && state.currentOp <= |tx.ops|
+                    && state.currentOp >= -1
+                    && if (state.currentOp >= 0 && state.currentOp < |tx.ops|) then (
+                        // Read/Write operations have at most two subOps
+                        state.currentSubOp < 2
+                    ) else if state.currentOp == |tx.ops| then (
+                        // tryCommit has 4 subOps
+                        state.currentSubOp < 4
+                    ) else if state.currentOp == -1 then (
+                        // abort has 3 subOps
+                        state.currentSubOp < 3
+                    ) else false
+                )
+                && state.readSet.Keys <= objValues.Keys
+                && state.writeSet.Keys <= objValues.Keys
+            ) else false
+        }
+
+        predicate validSystem()
+        {
+            && procStates.Keys <= txQueues.Keys
+            && objValues.Keys == objTimeStamps.Keys
+            && lockedObjs <= objValues.Keys
+            && forall p, s :: p in procStates && s == procStates[p] ==> stateValid(p, s)
+        }
+    }
+    
+
+    method Step(input: TMSystem, pid: ProcessId) returns (system: TMSystem)
+        requires pid in input.txQueues
+        requires pid in input.procStates
+        requires input.validSystem()
+        ensures system.validSystem()
+    {
+        system := input;
+        var state: ProcessState := system.procStates[pid];
+        assert(system.stateValid(pid, state)); // Given by input.validSystem()
+        var txs := system.txQueues[pid];
+
+        if (state.currentTx >= |txs|) {
+            // Nothing left to do.
+            return;
+        }
+        var tx := txs[state.currentTx];
+        
+        if (state.currentOp == |tx.ops|) {
+            // tryCommit
+            if(state.currentSubOp == 0) {
+                // Validate timestamps
+                if !(forall o :: o in state.readSet ==> state.readSet[o] == system.objTimeStamps[o]) {
+                    // Write detected (timestamp changed), aborting.
+                    state := new ProcessState.abortTx(state);
+                    system := new TMSystem.updateState(system, pid, state);
+                    assume(system.validSystem()); // TODO : Remove assumption.
+                    return;
                 }
-            } else if (state.currentOp == -1) {
-                // Abort
+                // Continue to next sub-op.
+                state := new ProcessState.nextSubOp(state);
+            } else if (state.currentSubOp == 1) {
+                // Check locks
+                if !(forall o :: o in state.readSet ==> o in state.writeSet || o !in system.lockedObjs) {
+                    // Write detected (locked), aborting.
+                    state := new ProcessState.abortTx(state);
+                    system := new TMSystem.updateState(system, pid, state);
+                    assume(system.validSystem()); // TODO : Remove assumption.
+                    return;
+                }
+                // Can commit ! Continue to next sub-op.
+                state := new ProcessState.nextSubOp(state);
+            } else if (state.currentSubOp == 2) {
+                // Update timestamps
+                system := new TMSystem.updateTimestamps(system, state.writeSet.Keys);
+                // Continue to next sub-op.
+                state := new ProcessState.nextSubOp(state);
+            } else if (state.currentSubOp == 3) {
+                // Release locks
+                system := new TMSystem.releaseLocks(system, state.writeSet.Keys);
+                // Commited. Continue to next transaction.
+                state := new ProcessState.nextTx(state);
+            } else {
+                assert(false);
+            }
+        } else if (state.currentOp == -1) {
+            // Abort
+            if(state.currentSubOp == 0) {
+                assert(state.currentTx < |system.txQueues[pid]|);
+                // Restore written values
+                system := new TMSystem.restoreValues(system, state.writeSet);
+                // Continue to next sub-op.
+                state := new ProcessState.nextSubOp(state);
+            } else if (state.currentSubOp == 1) {
+                // Update timestamps
+                system := new TMSystem.updateTimestamps(system, state.writeSet.Keys);
+                // Continue to next sub-op.
+                state := new ProcessState.nextSubOp(state);
+            } else if (state.currentSubOp == 2) {
+                // Release locks
+                system := new TMSystem.releaseLocks(system, state.writeSet.Keys);
+                // Restart transaction.
+                state := new ProcessState.restartTx(state);
+            } else {
+                assert(false);
+            }
+        } else if (state.currentOp >= 0 && state.currentOp < |tx.ops|) {
+            // Read/Write op
+            var op := tx.ops[state.currentOp];
+            var o := op.memObject;
+            
+            // Init object value and timestamp if not present
+            if(o !in system.objValues || o !in system.objTimeStamps) {
+                system := new TMSystem.initValue(system, o);
+            }
+            assert(o in system.objValues);
+            assert(o in system.objTimeStamps);
+
+            if(op.isWrite) {
+                // Write
                 if(state.currentSubOp == 0) {
-                    // Reset written values
-                    objValues := map o | o in objValues ::
-                        if(o in state.writeSet) then state.writeSet[o] else objValues[o];
-                    // Continue to next sub-op.
-                    state.currentSubOp := state.currentSubOp + 1;
+                    if(!(op.memObject in state.writeSet)) {
+                        // trylock
+                        if(o in system.lockedObjs) {
+                            // Failed locking, aborting.
+                            state := new ProcessState.abortTx(state);
+                        } else {
+                            // Aquire lock. Continue to next sub-op.
+                            assert(o in system.objValues);
+                            system := new TMSystem.acquireLock(system, o);
+                            assert(o in system.objValues);
+                            state := new ProcessState.addToWriteSet(state, o, system.objValues[o]);
+                            state := new ProcessState.nextSubOp(state);
+                        }
+                    } else {
+                        // Already in writeset, continue to next subOp.
+                        state := new ProcessState.nextSubOp(state);
+                    }
                 } else if (state.currentSubOp == 1) {
-                    // Update timestamps
-                    objTimeStamps := map o | o in objTimeStamps ::
-                        if(o in state.writeSet) then (objTimeStamps[o] + 1) else objTimeStamps[o];
-                    // Continue to next sub-op.
-                    state.currentSubOp := state.currentSubOp + 1;
-                } else if (state.currentSubOp == 2) {
-                    // Release locks
-                    lockedObjs := lockedObjs - state.writeSet.Keys;
-                    state.writeSet := map[];
-                    state.readSet := map[];
-                    // Restart transaction.
-                    state.currentOp := 0;
-                    state.currentSubOp := 0;
+                    // Do the write (simple increment). Continue to next op.
+                    system := new TMSystem.updateValue(system, o, system.objValues[o] + 1);
+                    state := new ProcessState.nextOp(state);
+                } else {
+                    assert(false);
                 }
             } else {
-                assert state.currentOp >= 0 && state.currentOp < |tx.ops|;
-                var op := tx.ops[state.currentOp];
-                var o := op.memObject;
-                
-                // Init values
-                if(o !in objValues) {
-                    objValues := objValues[o := 0];
-                }
-                if(o !in objTimeStamps) {
-                    objTimeStamps := objTimeStamps[o := 0];
-                }
-
-                if(op.isWrite) {
-                    // Write
-                    if(state.currentSubOp == 0) {
-                        if(!(op.memObject in state.writeSet)) {
-                            // trylock
-                            if(o in lockedObjs) {
-                                // Failed locking, aborting.
-                                state.currentOp := -1;
-                                state.currentSubOp := 0;
-                                return;
-                            } else {
-                                // Aquire lock. Continue to next sub-op.
-                                lockedObjs := lockedObjs + {o};
-                                state.writeSet := state.writeSet[o := objValues[o]];
-                            }
-                        }
-                        state.currentSubOp := state.currentSubOp + 1;
-                    } else if (state.currentSubOp == 1) {
-                        // Do the write (simple increment). Continue to next op.
-                        objValues := objValues[o := (objValues[o] + 1)];
-                        state.currentOp := state.currentOp + 1;
-                        state.currentSubOp := 0;
+                // Read operation
+                if(state.currentSubOp == 0) {
+                    if(o in state.writeSet || o in state.readSet) {
+                        // Already in writeSet or readSet, fast-skip to next op.
+                        state := new ProcessState.nextOp(state);
+                    } else {
+                        // Read timestamp and add to readSet. Continue to next sub-op.
+                        state := new ProcessState.addToReadSet(state, o, system.objTimeStamps[o]);
+                        state := new ProcessState.nextSubOp(state);
+                    }
+                } else if (state.currentSubOp == 1) {
+                    if(o in system.lockedObjs) {
+                        // Object is locked, aborting.
+                        state := new ProcessState.abortTx(state);
+                    } else {
+                        // All good. Continue to next op.
+                        state := new ProcessState.nextOp(state);
                     }
                 } else {
-                    // Read operation
-                    if(state.currentSubOp == 0) {
-                        if(o in state.writeSet || o in state.readSet) {
-                            // Already in writeSet or readSet, fast-skip to next op.
-                            state.currentOp := state.currentOp + 1;
-                            state.currentSubOp := 0;
-                            return;
-                        }
-                        // Read timestamp and add to readSet. Continue to next sub-op.
-                        state.readSet := state.readSet[o := objTimeStamps[o]];
-                        state.currentSubOp := state.currentSubOp + 1;
-                    } else if (state.currentSubOp == 1) {
-                        if(o in lockedObjs) {
-                            // Object is locked, aborting.
-                            state.currentOp := -1;
-                            state.currentSubOp := 0;
-                        } else {
-                            // All good. Continue to next op.
-                            state.currentOp := state.currentOp + 1;
-                            state.currentSubOp := 0;
-                        }
-                    }
+                    assert(false);
                 }
             }
+        } else {
+            assert(false);
         }
+        // Save the new state.
+        system := new TMSystem.updateState(system, pid, state);
+        assume(system.validSystem()); // TODO : Remove assumption.
     }
 }
